theories/approxis/examples/prf_cpa_combined_sem_typ.v
@@ -1,0 +1,1276 @@
+From clutch.prob_lang.typing Require Import tychk.
+From clutch.approxis Require Import approxis map list.
+From clutch.approxis.examples Require Import prf symmetric (* prf_cpa *) security_aux xor advantage.
+Set Default Proof Using "Type*".
+
+Section combined.
+
+  (*** A PRF *)
+
+  (** PRF Parameters. *)
+  Variable Key : nat.
+  Variable Input : nat.
+  Variable Output : nat.
+
+  Definition q_calls := q_calls_poly Input.
+
+  Definition N := S Input.
+
+
+  Definition q_calls_poly : val :=
+    Λ: Λ: λ:"Q" "f",
+      let: "counter" := ref #0 in
+      λ:"x", if: (! "counter" < "Q")
+             then ("counter" <- !"counter" + #1 ;; SOME ("f" "x"))
+             else NONEV.
+
+  Definition PRF_real : val :=
+    let keygen PRF_scheme : expr := Fst PRF_scheme in
+    let prf PRF_scheme : expr := Fst (Snd PRF_scheme) in
+    λ:"PRF_scheme" "Q",
+      let: "k" := keygen "PRF_scheme" #() in
+      let: "lookup" := prf "PRF_scheme" "k" in
+      let: "oracle" := q_calls_poly #() #() "Q" "lookup" in
+      "oracle".
+
+  Definition PRF_rand : val :=
+    let rand_output PRF_scheme : expr := Snd (Snd PRF_scheme) in
+    λ:"PRF_scheme" "Q",
+      let: "lookup" := random_function Output #() in
+      let: "oracle" := q_calls_poly #() #() "Q" "lookup" in
+      "oracle".
+
+  (** PRF Security: Local instances of the PRF games. **)
+  (* Definition PRF_rand := PRF_rand Input Output.
+     Definition PRF_real := PRF_real Input. *)
+  (* Max number of oracle calls *)
+  Variable (Q : nat).
+
+  Let ε_Q := (INR Q * INR Q / (2 * INR (S Input)))%R.
+
+  Local Opaque INR.
+
+  (** The PRF: (keygen, F, rand_output) *)
+  Variable keygen : val.
+  Variable F : val.
+  Definition rand_output : val := λ:"_", rand #Output.
+
+  Definition PRF_scheme_F : val := (keygen, (F, rand_output)).
+
+  (** RandML types: PRF and PRF adversary *)
+  Definition TKey := TNat.
+  Definition TInput := TNat.
+  Definition TOutput := TNat.
+  Definition TKeygen : type := (TUnit → TKey)%ty.
+  Definition TPRF : type := TKey → TInput → TOutput.
+
+  Definition T_PRF_Adv := ((TInput → (TOption TOutput)) → TBool)%ty.
+
+  Definition lrel_int_bounded {Σ} min max : lrel Σ := LRel (λ w1 w2, ∃ k : Z, ⌜ w1 = #k ∧ w2 = #k ∧ min <=k ∧ k <= max ⌝)%Z%I.
+
+  Definition lrel_key {Σ} : lrel Σ := lrel_int_bounded 0 Key.
+  Definition lrel_input {Σ} : lrel Σ := lrel_int_bounded 0 Input.
+  Definition lrel_output {Σ} : lrel Σ := lrel_int_bounded 0 Output.
+  Definition lrel_keygen `{!approxisRGS Σ} : lrel Σ := (lrel_unit → lrel_key).
+  Definition lrel_prf `{!approxisRGS Σ} : lrel Σ := lrel_key → lrel_input → lrel_output.
+
+  Definition lrel_option {Σ} (A : lrel Σ) := (() + A)%lrel.
+
+  Definition lrel_PRF_Adv `{!approxisRGS Σ} := ((lrel_input → (lrel_option lrel_output)) → lrel_bool)%lrel.
+
+  (** Assumption: the PRF is typed. *)
+  (* TODO: The type TPRF requires F to be safe for all inputs ; maybe this
+     assumption is unrealistic, and F should only be required to be safe only
+     for inputs in {0..Key}x{0..Input}. *)
+  Hypothesis F_typed : (⊢ᵥ F : TPRF).
+  Hypothesis keygen_typed : (⊢ᵥ keygen : TKeygen).
+  Hypothesis F_sem_typed : forall `{!approxisRGS Σ}, (⊢ REL F << F : lrel_prf).
+  Hypothesis keygen_sem_typed : forall `{!approxisRGS Σ}, (⊢ REL keygen << keygen : lrel_keygen).
+
+
+  (*** Symmetric scheme sym_scheme_F based on the PRF **)
+  (** Symmetric Scheme Parameters **)
+  Let Message := Output.
+  Let Cipher := Input * Output.
+
+  (** Security for Symmetric Encryption *)
+  (* Let CPA_real := CPA_real Message.
+     Let CPA_rand := CPA_rand Message. *)
+
+  Definition CPA_real : val :=
+    let keygen scheme : expr := Fst scheme in
+    let enc scheme : expr := Fst (Snd scheme) in
+    λ:"scheme" "Q",
+      let: "key" := keygen "scheme" #() in
+      q_calls_poly #() #() "Q" (enc "scheme" "key").
+
+  Definition CPA_rand : val :=
+    let rand_cipher scheme : expr := Snd (Snd scheme) in
+    λ:"scheme" "Q",
+      q_calls_poly #() #() "Q" (rand_cipher "scheme").
+
+  (** RandML typing *)
+  Definition TMessage := TInt.
+  Definition TCipher := (TInput * TOutput)%ty.
+  Definition lrel_message {Σ} : lrel Σ := lrel_int_bounded 0 Message.
+  Definition lrel_cipher {Σ} : lrel Σ := lrel_input * lrel_output.
+
+  (** Parameters required for the construction of sym_scheme_F *)
+  (* H_in_out is required to make sense of the assumption that xor is a bijection. *)
+  Hypothesis H_in_out : (Input = Output).
+  (* An abstract `xor`, in RandML and in Coq. *)
+  Context `{XOR Message Output}.
+  (* TODO relax typing of xor to be semantic *)
+
+  (** Generic PRF-based symmetric encryption. *)
+  (* Redefined here to make it parametrised by the PRF on the Coq level. *)
+  Definition prf_enc (prf : val) : val :=
+    λ:"key",
+      let: "prf_key" := prf "key" in
+      let: "α" := AllocTape #Input in
+      λ: "msg",
+        let: "r" := rand("α") #Input in
+        let: "z" := "prf_key" "r" in
+        ("r", xor "msg" "z").
+
+  Let F_keygen := keygen.
+  Definition F_enc : val := prf_enc F.
+  Definition F_rand_cipher : val := λ:<>, let:"i" := rand #Input in let:"o" := rand #Output in ("i", "o").
+  Definition sym_scheme_F : val := (F_keygen, (F_enc, F_rand_cipher)).
+
+  (** An IND$-CPA adversary. *)
+  Variable adversary : val.
+  Definition T_IND_CPA_Adv : type := (TMessage → TOption TCipher) → TBool.
+  (* Assumption: the adversary is typed. *)
+  Hypothesis adversary_typed : (⊢ᵥ adversary : T_IND_CPA_Adv).
+
+  Definition lrel__IND_CPA_Adv `{!approxisRGS Σ} : lrel Σ :=
+    (lrel_message → lrel_option lrel_cipher) → lrel_bool.
+  (* Assumption: the adversary is semantically typed. *)
+  Hypothesis adversary_sem_typed : forall `{!approxisRGS Σ},
+      (⊢ REL adversary << adversary : lrel__IND_CPA_Adv).
+
+  Definition opt_mult_poly : val :=
+    Λ: λ:"opt",
+      match: "opt" with
+      | NONE => NONE
+      | SOME "vopt" =>
+          match: "vopt" with
+          | NONE => NONE
+          | SOME "v" => SOME "v"
+          end
+      end.
+
+  Fact opt_mult_poly_typed : (⊢ᵥ opt_mult_poly : ∀: (TOption (TOption #0) → TOption #0)%ty).
+  Proof.
+    rewrite /opt_mult_poly. constructor. tychk.
+  Qed.
+
+  (** The reduction to PRF security. *)
+  Definition R_prf : val :=
+    λ:"prf_key",
+      let: "prf_key_q" := q_calls_poly #() #() #Q
+                     (λ: "msg",
+                        let: "r" := rand #Input in
+                        let: "z" := "prf_key" "r" in
+                        match: "z" with
+                        | SOME "z" => SOME ("r", xor "msg" "z")
+                        | NONE => NONE
+                        end
+                     ) in
+      λ:"msg", opt_mult_poly #() ("prf_key_q" "msg").
+
+  (** without q_calls *)
+  Definition R_prf' : val :=
+    λ:"prf_key",
+      (* let: "prf_key_q" :=
+           q_calls_poly #() #() #Q *)
+      let: "α" := AllocTape #Input in
+                     (λ: "msg",
+                        let: "r" := rand("α") #Input in
+                        let: "z" := "prf_key" "r" in
+                        match: "z" with
+                        | SOME "z" => SOME ("r", xor "msg" "z")
+                        | NONE => NONE
+                        end
+                     )
+      (* in
+         λ:"msg", opt_mult_poly #() ("prf_key_q" "msg") *)
+  .
+
+  Definition RED : val :=
+    λ:"prf_key", adversary (R_prf "prf_key").
+
+  Definition RED' : val :=
+    λ:"prf_key", adversary (R_prf' "prf_key").
+
+  Fact red_typed : (⊢ᵥ RED : T_PRF_Adv).
+  Proof.
+    rewrite /RED. tychk. 1: eauto.
+    rewrite /R_prf. constructor.
+    type_expr 4.
+    all: try by tychk.
+    3: tychk ; apply xor_typed.
+    2: rewrite /q_calls /q_calls_poly.
+    2: tychk.
+    rewrite /opt_mult_poly. tychk.
+  Qed.
+
+  Hypothesis xor_sem_typed : forall `{!approxisRGS Σ} (Key Support : nat) (xor_struct : @XOR Key Support),
+    ⊢ (lrel_int_bounded 0 Key → lrel_int_bounded 0 Support → lrel_int_bounded 0 Support)%lrel
+        (@xor _ _ xor_struct) (@xor _ _ xor_struct).
+
+  Hypothesis refines_tape_couple_avoid : forall `{!approxisRGS Σ} (N:nat) α l z E K K' A,
+    NoDup l ->
+    TCEq N (Z.to_nat z) →
+    ↯ (length l / (S N)) ∗
+    α ↪N (Input; []) ∗
+    ▷ (∀ (n : fin (S N)), ⌜n ∉ l⌝ -∗ α ↪N (Input; []) -∗ REL fill K (Val #n) << fill K' (Val #n) @ E : A)
+    ⊢ REL fill K (rand(#lbl:α) #z) << fill K' (rand #z) @ E : A.
+
+  Section approxis_proofs.
+
+  Context `{!approxisRGS Σ}.
+
+(*   Section compat_aux.
+       Implicit Types Δ : listO (lrelC Σ).
+       Hint Resolve to_of_val : core.
+
+       Local Ltac intro_clause := progress (iIntros (vs) "#Hvs /=").
+       Local Ltac intro_clause' := progress (iIntros (?) "? /=").
+       Local Ltac value_case := try intro_clause';
+                                try rel_pure_l; try rel_pure_r; rel_values.
+
+   Section bin_log_related_sem.
+     Context `{!approxisRGS Σ}.
+
+     Definition bin_log_related_sem (E : coPset)
+                (Δ : list (lrel Σ)) (Γ : stringmap type)
+                (e e' : expr) (τ : lrel Σ) : iProp Σ :=
+       (∀ vs, ⟦ (λ τ, interp τ Δ) <$> Γ ⟧* vs -∗
+              REL (subst_map (fst <$> vs) e)
+               << (subst_map (snd <$> vs) e') @ E : τ)%I.
+
+   End bin_log_related_sem.
+
+       Local Tactic Notation "rel_bind_ap" uconstr(e1) uconstr(e2) constr(IH) ident(v) ident(w) constr(Hv):=
+         rel_bind_l (subst_map _ e1);
+         rel_bind_r (subst_map _ e2);
+         try iSpecialize (IH with "Hvs");
+         iApply (refines_bind with IH);
+         iIntros (v w) Hv; simpl.
+
+       Lemma bin_log_related_rec Δ (Γ : stringmap type) (f x : binder) (e e' : expr) τ1 τ2 :
+         □ (〈Δ;<[f:=lrel_arr τ1 τ2]>(<[x:=τ1]>Γ)〉 ⊨ e ≤log≤ e' : τ2) -∗
+         〈Δ;Γ〉 ⊨ Rec f x e ≤log≤ Rec f x e' : τ1 → τ2.
+       Proof.
+         iIntros "#Ht".
+         intro_clause.
+         rel_pure_l. rel_pure_r.
+         iApply refines_arrow_val.
+         iModIntro. iLöb as "IH". iIntros (v1 v2) "#Hτ1".
+         rel_pure_l. rel_pure_r.
+
+         set (r := (RecV f x (subst_map (binder_delete x (binder_delete f (fst <$> vs))) e), RecV f x (subst_map (binder_delete x (binder_delete f (snd <$> vs))) e'))).
+         set (vvs' := binder_insert f r (binder_insert x (v1,v2) vs)).
+         iSpecialize ("Ht" $! vvs' with "[#]").
+         { rewrite !binder_insert_fmap.
+           iApply (env_ltyped2_insert with "[IH]").
+           - iApply "IH".
+           - iApply (env_ltyped2_insert with "Hτ1").
+             by iFrame. }
+
+         unfold vvs'.
+         destruct x as [|x], f as [|f];
+                             rewrite /= ?fmap_insert ?subst_map_insert //.
+         try by iApply "H".
+         destruct (decide (x = f)) as [->|]; iSimpl in "Ht".
+         - rewrite !delete_insert_delete !subst_subst !delete_idemp.
+           by iApply "Ht".
+         - rewrite !delete_insert_ne // subst_map_insert.
+           rewrite !(subst_subst_ne _ x f) // subst_map_insert.
+           by iApply "Ht".
+       Qed.
+
+     End compat_aux. *)
+
+  Fact opt_mult_poly_sem_typed :
+    ⊢ (∀ A : lrel Σ, lrel_option (lrel_option A) → lrel_option A)%lrel
+      opt_mult_poly opt_mult_poly.
+  Proof.
+    replace (∀ A : lrel Σ, lrel_option (lrel_option A) → lrel_option A)%lrel
+      with (interp (∀: TOption (TOption #0) → TOption #0) []) by easy.
+    iApply fundamental_val.
+    rewrite /opt_mult_poly. constructor. tychk.
+  Qed.
+
+  Fact q_calls_poly_sem_typed :
+    ⊢ (∀ A B : lrel Σ, lrel_int → (A → B) → A → lrel_option B)%lrel
+        q_calls_poly q_calls_poly.
+  Proof.
+    replace (∀ A B : lrel Σ, lrel_int → (A → B) → A → lrel_option B)%lrel
+      with (interp (∀: ∀: TInt → (#1 → #0) → #1 → TOption #0) []) by easy.
+    iApply fundamental_val.
+    rewrite /q_calls_poly. do 3 constructor. tychk.
+  Qed.
+
+  Fact red_sem_typed : (⊢ REL RED <<  RED : lrel_PRF_Adv).
+  Proof using (xor_sem_typed adversary_sem_typed
+H_in_out) with (rel_pures_r ; rel_pures_l).
+    rel_arrow ; iIntros (f f') "#hff'" ; rel_pures_l ; rel_pures_r.
+    unfold RED...
+    rel_apply refines_app => //.
+    1: iApply adversary_sem_typed.
+    rewrite /R_prf...
+    unshelve rel_apply refines_app => //.
+    1: exact (lrel_input → lrel_option (lrel_option lrel_cipher))%lrel.
+    - rel_arrow. iIntros (??) "#?"...
+      rel_arrow_val. iIntros (??) "#(%mm&->&->&%&%)"...
+      rel_apply (refines_app _ _ _ _ (lrel_option (lrel_option lrel_cipher))) => //.
+      + by iApply (opt_mult_poly_sem_typed $! lrel_cipher).
+      + rel_apply refines_app. 1: done.
+        rel_values. iExists _. iModIntro ; repeat iSplit ; try by easy.
+        rewrite H_in_out. done.
+    -
+      unshelve rel_apply refines_app => //.
+      1: exact (lrel_input → lrel_option lrel_cipher)%lrel.
+      1: {
+        rel_apply refines_app. 2: iApply refines_typed ; tychk. simpl.
+        iPoseProof (q_calls_poly_sem_typed $! lrel_input #() #() _) as "bla".
+        rel_bind_l (q_calls_poly #()). rel_bind_r (q_calls_poly #()).
+        rel_apply refines_bind.
+        1: iApply "bla".
+        iIntros (??) "#foo".
+        iApply ("foo" $! (lrel_option lrel_cipher)) => //.
+      }
+      rel_arrow_val ; iIntros (??) "(%msg & -> & -> & % & %)"...
+      rel_bind_l (rand _)%E. rel_bind_r (rand _)%E. rel_apply (refines_bind _ _ _ lrel_input).
+      { rel_apply (refines_couple_UU Input id); first auto. iModIntro. iIntros. rel_values.
+        iExists _. iPureIntro ; repeat split ; lia. }
+      iIntros (??) "(%r&->&->&%&%)"...
+      rel_bind_l (f _). rel_bind_r (f' _). rel_apply refines_bind.
+      { rel_apply refines_app. 1: done.
+        rel_values. iExists _. iPureIntro ; repeat split ; try rewrite H_in_out ; try lia. }
+      iIntros (??) "#(%zopt&%zopt'&[(->&->&?) | (->&->&ttt)])"...
+      1: rel_values ; iExists _, _ ; iLeft ; iPureIntro ; repeat split.
+      rel_bind_l (xor _ _). rel_bind_r (xor _ _). rel_apply refines_bind.
+      { repeat rel_apply refines_app.
+        1: rel_values ; iApply xor_sem_typed.
+        all: rel_values. iExists _. iPureIntro ; repeat split ; lia. }
+      iIntros (??) "(%c&->&->&%&%)"...
+      rel_values.
+      iExists _,_ ; iRight ; iPureIntro ; repeat (try split ; try eexists _) ; lia.
+      Unshelve. 2: done. exact [].
+  Qed.
+
+  Fact red_sem_typed' : (⊢ REL RED' <<  RED' : lrel_PRF_Adv).
+  Proof using (xor_sem_typed adversary_sem_typed
+H_in_out) with (rel_pures_r ; rel_pures_l).
+    rel_arrow ; iIntros (f f') "#hff'" ; rel_pures_l ; rel_pures_r.
+    unfold RED'...
+    rel_apply refines_app => //.
+    1: iApply adversary_sem_typed.
+    rewrite /R_prf'...
+
+    rel_alloctape_l α as "α".
+    rel_alloctape_r α' as "α'"...
+
+    iApply (refines_na_alloc
+              ( α ↪N (Input; [])
+                             ∗ α' ↪ₛN (Input; [])
+                             (* ∗ counter_r' ↦ₛ #q *) )%I
+              (nroot.@"tapes")) ; iFrame.
+      (* iSplitL. 1: done. *)
+
+      iIntros "#Hinv".
+
+    (* unshelve rel_apply refines_app. 1: exact (interp TTape []).
+       2:{ rel_apply refines_typed. simpl. tychk. } *)
+    (* rel_arrow_val ; iIntros (??) "(% & % & % & -> & -> & #hh)"... *)
+
+      rel_arrow_val ; iIntros (??) "(%msg & -> & -> & % & %)"...
+      rel_bind_l (rand(_) _)%E. rel_bind_r (rand(_) _)%E. rel_apply (refines_bind _ _ _ lrel_input).
+      {
+      (* rel_arrow_val. *)
+      (* iIntros (??) "#(%msg&->&->&%&%)"... *)
+      iApply (refines_na_inv with "[$Hinv]"); [done|].
+      iIntros "(> (α & α') & Hclose)".
+        (* iMod (inv_acc with "hh") as "[>hhh Hclose]"; [done|].
+           iInv (logN.@(α1, α2)) as "HI". *)
+      iMod ec_zero.
+        rel_apply (refines_couple_TT_err Input Input _ _ _ _ _ _ _ _ 0%R); first auto.
+        1: lra.
+        iFrame. iIntros (?) "(?&?&%)"...
+        rel_apply (refines_rand_r with "[$]").
+        iIntros "α' %".
+        rel_apply (refines_rand_l).
+        iFrame. iIntros "!> α %".
+        iApply (refines_na_close with "[-]") ; iFrame ; iFrame.
+        rel_values ; iExists _ ; iPureIntro ; repeat split ; lia. }
+
+      iIntros (??) "(%r&->&->&%&%)"...
+      rel_bind_l (f _). rel_bind_r (f' _). rel_apply refines_bind.
+      { rel_apply refines_app. 1: done.
+        rel_values. iExists _. iPureIntro ; repeat split ; try rewrite H_in_out ; try lia. }
+      iIntros (??) "#(%zopt&%zopt'&[(->&->&?) | (->&->&ttt)])"...
+      1: rel_values ; iExists _, _ ; iLeft ; iPureIntro ; repeat split.
+      rel_bind_l (xor _ _). rel_bind_r (xor _ _). rel_apply refines_bind.
+      { repeat rel_apply refines_app.
+        1: rel_values ; iApply xor_sem_typed.
+        all: rel_values. iExists _. iPureIntro ; repeat split ; lia. }
+      iIntros (??) "(%c&->&->&%&%)"...
+      rel_values.
+      iExists _,_ ; iRight ; iPureIntro ; repeat (try split ; try eexists _) ; lia.
+  Qed.
+
+
+  Lemma reduction :
+    ⊢ (REL (adversary (CPA_real sym_scheme_F #Q))
+         << (RED' (PRF_real PRF_scheme_F #Q)) : lrel_bool).
+  Proof using (xor_sem_typed adversary_sem_typed H_in_out keygen_sem_typed Key F_sem_typed)
+    with (rel_pures_l ; rel_pures_r).
+    rewrite /PRF_scheme_F/PRF_real/prf.PRF_real.
+    rel_pures_r.
+    rewrite /CPA_real/symmetric.CPA_real.
+    rel_pures_l. rewrite /F_keygen.
+    rel_bind_l (keygen _)%E.
+    rel_bind_r (keygen _)%E.
+    unshelve iApply (refines_bind with "[-] []").
+    1: exact lrel_key.
+    1: rel_apply refines_app ; [iApply keygen_sem_typed|by rel_values].
+    iIntros (??(key&->&->&?&?)) => /=...
+    rewrite /F_enc/prf_enc...
+    rel_bind_l (F #key)%E. rel_bind_r (F #key)%E.
+    unshelve iApply (refines_bind with "[-] []").
+    1: exact (lrel_input → lrel_output)%lrel.
+    1: rel_apply refines_app ; [iApply F_sem_typed|].
+    1: rel_values ; iExists _ ; easy.
+    iIntros (F_key F_key') "#rel_prf_key".
+    simpl...
+    rewrite {2}/q_calls_poly. rel_pures_r.
+    rel_alloc_r counter_r as "counter_r"...
+    rewrite /RED'. rel_pures_r.
+    rel_bind_l (q_calls_poly _ _ _ _)%E.
+    rel_bind_r (R_prf' _)%E.
+    unshelve iApply (refines_bind with "[-] []").
+    1: exact (lrel_message → lrel_option lrel_cipher)%lrel.
+    2:{ simpl. iIntros (f f') "H_f_f'".
+        rel_pures_r.
+        iApply refines_app. 2: rel_values.
+        iApply adversary_sem_typed.
+    }
+    simpl.
+    rewrite /R_prf'...
+    rewrite /q_calls_poly...
+
+    rel_alloctape_l α as "α".
+    rel_alloctape_r α' as "α'"...
+
+    rel_alloc_l counter_l as "counter_l".
+    rel_pures_l ; rel_pures_r.
+    (* Invariant: all counters agree. *)
+    iApply (refines_na_alloc
+              ( ∃ (q : nat) xs ys, counter_l ↦ #q
+                                   ∗ counter_r ↦ₛ #q
+                                   ∗ (α ↪N (Input; xs))
+                                   ∗ (α' ↪ₛN (Input; []))
+                                   ∗ (⌜(q < Q)%Z⌝ -∗ ⌜xs = [] ∧ ys = []⌝)
+              )%I
+              (nroot.@"RED")).
+    iSplitL.
+    1: iExists 0 ; iFrame "counter_r counter_l" ; iFrame ; try done.
+    1: iExists [] ; done.
+
+    iIntros "#Hinv".
+    rel_arrow_val.
+    iIntros (??) "#(%msg&->&->&%&%)"...
+    iApply (refines_na_inv with "[$Hinv]"); [done|].
+    iIntros "(> (%q & %xs & %ys & counter_l & counter_r & α & α' & HqQ) & Hclose)".
+
+    destruct_decide (@bool_decide_reflect (q < Q)%Z _) as qQ.
+
+    - iDestruct ("HqQ" $! _) as "(-> & ->)".
+
+      iMod ec_zero.
+      rel_apply (refines_couple_TT_err Input Input _ _ _ _ _ _ _ _ 0%R) ; [auto|lra|].
+      iFrame. iIntros (r) "(α&?&%)"...
+      rel_apply (refines_rand_r with "[$]")...
+      iIntros "α' %"...
+
+      rel_load_l ; rel_load_r...
+
+      case_bool_decide as qQ'...
+      2: by exfalso.
+
+      rel_load_l. rel_load_r... rel_store_l ; rel_store_r...
+      rel_apply_l (refines_rand_l with "[-$α]")...
+      iIntros "!> α %"...
+      iApply (refines_na_close with "[-]") ; iFrame ; iFrame.
+      iSplitL.
+      { iExists (q+1), []. iNext. iFrame.
+        replace (Z.of_nat q + 1)%Z with (Z.of_nat (q+1)) by lia.
+        iFrame. done. }
+
+      rel_bind_l (F_key #r)%E.
+      rel_bind_r (F_key' #r)%E.
+      iApply (refines_bind with "[-] []") => /=.
+      { iApply "rel_prf_key". iExists _. iPureIntro ; repeat split ; lia. }
+      iIntros (??) "#(%z&->&->&%&%)"...
+      rel_bind_l (xor _ _)%E. rel_bind_r (xor _ _)%E.
+      iApply (refines_bind _ _ _ lrel_output with "[-] []") => /=.
+      { repeat rel_apply refines_app ; rel_values.
+        1: iApply xor_sem_typed.
+        all: iExists _ ; iPureIntro ; repeat split ; lia. }
+      iIntros (??) "(% & -> & -> & % & %)"... rel_values.
+      iExists _,_ ; iRight ; iPureIntro ; repeat (try split ; try eexists _) ; lia.
+
+    - rel_apply (refines_randT_empty_r with "[-$α']").
+      iIntros (?) "α' %"...
+      rel_load_l ; rel_load_r...
+      case_bool_decide as qQ' ; [by exfalso|]...
+      iApply (refines_na_close with "[-]").
+      iFrame. iFrame. rel_values. iExists _,_. iLeft. done.
+      Unshelve. 1: exact nat. done.
+  Qed.
+
+  Definition I := random_function Output.
+  Definition PRF_scheme_I := (λ:"_", #(), (I, rand_output))%V.
+
+  Fact q_calls_typed_int (MAX : Z) :
+    (⊢ᵥ (Λ: bounded_oracle.q_calls MAX) : ∀: (TInt → (TInt → #0) → TInt → TOption #0))%ty.
+  Proof.
+    rewrite /bounded_oracle.q_calls.
+    apply TLam_val_typed.
+    tychk.
+  Qed.
+
+  (* Should be just syntactic since PRF_rand doesn't use the PRF. *)
+  Lemma F_I :
+    ⊢ (REL (RED' (PRF_rand PRF_scheme_F #Q))
+         << (RED' (PRF_rand PRF_scheme_I #Q)) : lrel_bool).
+  Proof with (rel_pures_l ; rel_pures_r).
+    rewrite /PRF_scheme_F/PRF_scheme_I/PRF_rand/prf.PRF_rand...
+    rel_apply refines_app.
+    1: iApply red_sem_typed'.
+    unshelve rel_apply refines_app.
+    1: exact (lrel_input → lrel_output)%lrel.
+    - rel_arrow. iIntros (rf rf') "#hrf"...
+      unshelve rel_apply refines_app => //.
+      1: exact (lrel_input → lrel_option lrel_output)%lrel.
+      { rel_arrow. iIntros... done. }
+      unshelve rel_apply refines_app => //.
+      rel_apply refines_app. 2: iApply refines_typed ; tychk. simpl.
+      iPoseProof (q_calls_poly_sem_typed $! lrel_input #() #() _) as "bla".
+      rel_bind_l (q_calls_poly #()). rel_bind_r (q_calls_poly #()).
+      rel_apply refines_bind.
+      1: iApply "bla".
+      iIntros (??) "#foo".
+      iApply ("foo" $! lrel_output) => //.
+    - rewrite /random_function...
+      rewrite /init_map...
+      rewrite /init_list...
+      rel_alloc_l ? as "?". rel_alloc_r ? as "?".
+      rel_alloc_l ? as "?". rel_alloc_r ? as "?"...
+
+
+  (*     rel_bind_l (init_map _)%E. rel_bind_r (init_map _)%E. rel_apply refines_bind.
+         { rel_apply refines_app.
+           1: replace (_ → _)%lrel with (interp (TUnit → TMap TInt TInt) []) by eauto.
+           2: rel_values ; eauto.
+           rel_apply refines_typed.
+           simpl. tychk. apply init_map_typed.
+         }
+         simpl.
+         iIntros
+         rel_arrow_val.
+
+       replace (lrel_input → lrel_option lrel_output)%lrel with (interp TBool []) by auto.
+       iApply refines_typed. unshelve tychk.
+       3: apply red_typed.
+       1: exact (TInput → TOutput)%ty.
+       2:{ rewrite /random_function.
+           tychk.
+           - eapply get_typed => //. constructor.
+           - apply set_typed => //.
+           - apply init_map_typed.
+       }
+       apply q_calls_typed_nat.
+     Qed. *)
+  Admitted.
+
+  Definition I_enc := prf_enc I.
+  Definition sym_scheme_I := (λ:"_", #(), (I_enc, F_rand_cipher))%V.
+
+  Lemma reduction' :
+    ⊢ (REL (RED' (PRF_rand PRF_scheme_I #Q))
+         << (adversary (CPA_real sym_scheme_I #Q)) : lrel_bool).
+  Proof
+    using (keygen_typed adversary_typed H_in_out
+refines_tape_couple_avoid
+F_typed
+xor_sem_typed keygen_sem_typed adversary_sem_typed Key F_sem_typed)
+    with (rel_pures_l ; rel_pures_r).
+    rewrite /PRF_scheme_I/sym_scheme_I/PRF_rand/prf.PRF_rand/CPA_real/symmetric.CPA_real...
+    rewrite /F_keygen.
+
+    rewrite /I_enc. rewrite /prf_enc. rewrite /RED'/R_prf'. rewrite /I...
+    rewrite /random_function...
+    rel_bind_r (init_map #())%E.
+    iApply refines_init_map_r => /=...
+    iIntros (map_r) "map_r".
+    rel_bind_l (init_map #())%E.
+    iApply refines_init_map_l.
+    iIntros (map_l) "map_l" => /=...
+    rewrite /q_calls_poly...
+    rel_alloctape_r α' as "α'"...
+    rel_alloc_r counter_r as "counter_r"...
+    rel_alloc_l counter_l as "counter_l"...
+    (* rel_alloc_l counter_l' as "counter_l'"... *)
+    rel_alloctape_l α as "α".
+    unshelve rel_apply refines_app.
+    (* 1: exact (lrel_message → lrel_option lrel_cipher)%lrel. *)
+    (* { exact (interp (TMessage → TOption TCipher) []). } *)
+    2: iApply adversary_sem_typed.
+    (* { replace (interp (TMessage → TOption TCipher) [] → lrel_bool)%lrel with (interp T_IND_CPA_Adv []) by easy.
+           iApply refines_typed. by tychk. } *)
+    (* more or less: (enc_prf rand_fun|Q)|Q = (enc_prf rand_fun)|Q *)
+    iApply (refines_na_alloc
+              ( ∃ (q : nat) (M : gmap nat val) (xs ys : list nat), counter_l ↦ #q
+                             (* ∗ counter_l' ↦ #q *)
+                             ∗ counter_r ↦ₛ #q
+                             ∗ map_list map_l M
+                             ∗ map_slist map_r M
+                             ∗ ⌜ ∀ y, y ∈ @map_img nat val (gmap nat val) _ (gset val) _ _ _ M → ∃ k : nat, y = #k ∧ k <= Output ⌝
+                             (* ∗ ⌜ size (dom M) = q ⌝ *)
+                             ∗ ⌜ ∀ x, x ∈ elements (dom M) -> (x < S Input)%nat ⌝
+                             ∗ (α ↪N (Input; []))
+                             ∗ (α' ↪ₛN (Input; ys))
+                             ∗ (⌜(q < Q)%Z⌝ -∗ ⌜xs = [] ∧ ys = []⌝)
+              )%I
+              (nroot.@"RED")) ; iFrame.
+      iSplitL.
+      1: { iExists 0 ; iFrame. iExists []. iPureIntro; split ; [|set_solver].
+           intros y hy. exfalso. clear -hy.
+           rewrite map_img_empty in hy.
+           opose proof (proj1 (elem_of_empty y)hy ). done.
+      }
+      iIntros "#Hinv".
+      rel_arrow_val.
+      iIntros (??) "#(%msg&->&->&%&%)" ; rel_pures_l ; rel_pures_r.
+      iApply (refines_na_inv with "[$Hinv]"); [done|].
+      iIntros "(> (%q & %M & %xs & %ys & counter_l & counter_r & map_l & map_r & %range_int & %dom_range & α & α' & hα) & Hclose)".
+
+    destruct_decide (@bool_decide_reflect (q < Q)%Z _) as qQ.
+
+    - iDestruct ("hα" $! _) as "(-> & ->)".
+
+      iMod ec_zero.
+      rel_apply (refines_couple_TT_err Input Input _ _ _ _ _ _ _ _ 0%R) ; [auto|lra|].
+      iFrame. iIntros (r) "(α&α'&%)"...
+      rel_apply (refines_rand_l with "[-$α]")...
+      iIntros "!> α %"...
+
+      rel_load_l ; rel_load_r...
+
+      case_bool_decide as qQ'...
+      2: by exfalso.
+
+      rel_load_l. rel_load_r... rel_store_l ; rel_store_r...
+      rel_apply_r (refines_rand_r with "[$α']")...
+      iIntros "α' %"...
+
+      rel_apply_r (refines_get_r with "[-map_r] [$map_r]").
+      iIntros (?) "map_r #->"...
+      rel_apply_l (refines_get_l with "[-map_l] [$map_l]").
+      iIntros (?) "map_l #->"...
+
+      destruct (M !! r) as [y |] eqn:r_fresh ...
+      1: {
+        iApply (refines_na_close with "[-]") ;
+        iFrame ; repeat iSplitL. 1: iExists (q+1).
+        { iFrame.
+          replace (Z.of_nat q + 1)%Z with (Z.of_nat (q+1)) by lia.
+          iExists []. iNext. iFrame.
+          iPureIntro. split. 2: set_solver. done.
+        }
+
+        opose proof (elem_of_map_img_2 M r y r_fresh) as hy.
+        destruct (range_int y hy) as [x [??]]. subst.
+
+
+      rel_bind_l (xor _ _)%E. rel_bind_r (xor _ _)%E.
+      iApply (refines_bind _ _ _ lrel_output with "[-] []") => /=.
+      { repeat rel_apply refines_app ; rel_values.
+        1: iApply xor_sem_typed.
+        all: iExists _ ; iPureIntro ; repeat split ; try eauto with lia. }
+      iIntros (??) "(% & -> & -> & % & %)"... rel_values.
+      iExists _,_ ; iRight ; iPureIntro ; repeat (try split ; try eexists _) ; lia.
+      }
+
+      rel_apply (refines_couple_UU Output id); first auto.
+      iIntros (y) "!> %"...
+
+      rel_apply_r (refines_set_r with "[-map_r] [$map_r]").
+      iIntros "map_r"...
+      rel_apply_l (refines_set_l with "[-map_l] [$map_l]").
+      iIntros "map_l"...
+      iApply (refines_na_close with "[-]") ;
+      iFrame ; repeat iSplitL. 1: iExists _ ; iFrame.
+      1: {
+        replace (Z.of_nat q + 1)%Z with (Z.of_nat (q+1)) by lia.
+        iExists _. iNext. iFrame. iPureIntro.
+           repeat split ; last first.
+           - rewrite -Forall_forall.
+             rewrite dom_insert.
+             rewrite elements_union_singleton.
+             + apply Forall_cons_2.
+               1: lia.
+               rewrite Forall_forall.
+               done.
+             + apply not_elem_of_dom_2. done.
+           - intros y' hy'.
+             opose proof (map_img_insert M r (#y)) as eq.
+             rewrite eq in hy'.
+             rewrite elem_of_union in hy'.
+             destruct hy'.
+             + exists y. set_solver.
+             + apply range_int.
+               opose proof (delete_subseteq M r) as h.
+               eapply map_img_delete_subseteq. done.
+      }
+
+      rel_bind_l (xor _ _)%E. rel_bind_r (xor _ _)%E.
+      iApply (refines_bind _ _ _ lrel_output with "[-] []") => /=.
+      { repeat rel_apply refines_app ; rel_values.
+        1: iApply xor_sem_typed.
+        all: iExists _ ; iPureIntro ; repeat split ; lia. }
+      iIntros (??) "(% & -> & -> & % & %)"... rel_values.
+      iExists _,_ ; iRight ; iPureIntro ; repeat (try split ; try eexists _) ; lia.
+
+    - rel_apply (refines_randT_empty_l with "[-$α]").
+      iIntros "!>" (?) "α %"...
+      rel_load_l ; rel_load_r...
+      case_bool_decide as qQ' ; [by exfalso|]...
+      iApply (refines_na_close with "[-]").
+      iFrame.
+      iSplitL.
+      { iFrame.
+        iNext.
+        iPureIntro. split. 2: set_solver. done.
+      }
+      rel_values. iExists _,_. iLeft. done.
+      Unshelve. all: eauto. all: apply _.
+  Qed.
+
+  (* This should be the result proven for the Approxis paper. *)
+  Lemma cpa_I `{!XOR_spec} :
+    ↯ ε_Q
+    ⊢ (REL (adversary (CPA_real sym_scheme_I #Q))
+         << (adversary (CPA_rand sym_scheme_I #Q)) : lrel_bool).
+  Proof
+    using (adversary_typed keygen_typed F_typed
+xor_sem_typed refines_tape_couple_avoid keygen_sem_typed adversary_sem_typed
+Key H_in_out
+F_sem_typed
+)
+    with (rel_pures_l ; rel_pures_r).
+    (* clear H_in_out. *)
+    iIntros "ε".
+    rewrite /CPA_real/CPA_rand.
+    rewrite /symmetric.CPA_real/symmetric.CPA_rand...
+    rewrite /F_rand_cipher.
+    rewrite /I_enc/I...
+    (* should be more or less the old proof. *)
+    rewrite /prf_enc...
+    rewrite /random_function...
+    rel_bind_l (init_map #())%E.
+    iApply refines_init_map_l.
+    iIntros (map_l) "map_l" => /=...
+    rewrite /q_calls_poly...
+    rel_alloc_r counter_r as "counter_r"...
+    rel_alloctape_l α as "α".
+    rel_alloc_l counter_l as "counter_l"...
+
+    rel_bind_l (λ:"x", _)%V.
+    rel_bind_r (λ:"x", _)%V.
+    unshelve iApply (refines_bind with "[-] []") => /=.
+    1: exact (lrel_message → lrel_option lrel_cipher)%lrel.
+
+    2:{
+      iIntros (f f') "Hff'".
+      simpl.
+      unshelve iApply (refines_app with "[] [Hff']").
+      3: rel_values.
+      iApply adversary_sem_typed.
+    }
+
+      iApply (refines_na_alloc
+                (∃ (q : nat) M,
+                    ↯ ((Q*Q-q*q) / (2 * S Input))
+                    ∗ counter_l ↦ #q
+                    ∗ counter_r ↦ₛ #q
+                    ∗ map_list map_l M
+                    ∗ ⌜ size (dom M) = q ⌝
+                    ∗ ⌜ ∀ x, x ∈ elements (dom M) -> (x < S Input)%nat ⌝
+                    ∗ α ↪N (Input; [])
+                )%I
+                (nroot.@"cpa")); iFrame.
+      iSplitL.
+      1: { iExists 0.
+           rewrite INR_0.
+           replace (Q*Q-0*0)%R with (Q*Q)%R by lra.
+           iFrame. iPureIntro; set_solver.
+      }
+      iIntros "#Hinv".
+      rel_arrow_val.
+      iIntros (??) "#(%msg&->&->&%&%)" ; rel_pures_l ; rel_pures_r.
+      iApply (refines_na_inv with "[$Hinv]"); [done|].
+      iIntros "(> (%q & %M & ε & counter & counter' & mapref & %dom_q & %dom_range & α) & Hclose)".
+      (* case_bool_decide as Hm. *)
+      - rel_load_l ; rel_load_r...
+        (* rewrite -bool_decide_and. *)
+        case_bool_decide as Hq.
+        + rel_load_l ; rel_load_r... rel_store_l ; rel_store_r...
+          assert (Z.to_nat msg < S Message) as Hmsg by lia.
+          pose proof nat_to_fin_list _ (elements(dom M)) dom_range as [l' Hl'].
+
+
+          rel_apply (refines_tape_couple_avoid _ α l').
+          { apply NoDup_fmap with fin_to_nat; first apply fin_to_nat_inj.
+            rewrite Hl'. apply NoDup_elements. }
+          replace (length l') with q; last first.
+          { erewrite <-fmap_length, Hl'.
+            by replace (length (elements (dom M))) with (size (dom M)).
+          }
+          pose proof pos_INR_S (Input).
+          assert (0<=q/S Input)%R.
+          { apply Rcomplements.Rdiv_le_0_compat; last done.
+            apply pos_INR. }
+          assert (0<=(Q * Q - (q+1)%nat * (q+1)%nat)/(2*S Input))%R.
+          { apply Rcomplements.Rdiv_le_0_compat; last lra.
+            rewrite -!mult_INR. apply Rle_0_le_minus.
+            apply le_INR. rewrite -Nat.square_le_mono. lia. }
+          iDestruct (ec_weaken _ (q/S Input+((Q * Q - (q + 1)%nat * (q + 1)%nat))/ (2 * S Input)) with "[$]") as "ε".
+          { split; first lra.
+            apply Rcomplements.Rle_minus_r.
+            rewrite Rminus_def -Rdiv_opp_l -Rdiv_plus_distr.
+            rewrite Rdiv_mult_distr.
+            rewrite !Rdiv_def.
+            apply Rmult_le_compat_r.
+            { apply Rlt_le. by apply Rinv_0_lt_compat. }
+            rewrite -Rcomplements.Rle_div_r; last lra.
+            trans ((q + 1)%nat * (q + 1)%nat-q*q)%R; last lra.
+            rewrite plus_INR.
+            replace (INR 1) with 1%R by done. lra.
+          }
+          iDestruct (ec_split with "[$]") as "[ε ε']"; [done|done|].
+          iFrame.
+          iIntros (r_in) "!> %r_fresh α"...
+          rel_apply_l (refines_get_l with "[-mapref] [$mapref]").
+          iIntros (?) "mapref #->"...
+          assert ((M !! fin_to_nat r_in) = None) as ->.
+          { apply not_elem_of_dom_1.
+            rewrite -elem_of_elements.
+            rewrite -Hl'.
+            intros K. apply elem_of_list_fmap_2_inj in K; last apply fin_to_nat_inj.
+            done.
+          }
+          simpl...
+          unshelve rel_apply (refines_couple_UU _ (@xor_sem _ _ H (Z.to_nat msg))) ;
+            [apply xor_bij|apply xor_dom => //|..].
+          iIntros (y) "!> %"...
+          rel_apply_l (refines_set_l with "[-mapref] [$mapref]").
+          iIntros "mapref"...
+          rel_bind_l (xor _ _).
+          rel_apply_l xor_correct_l; [done | lia | lia |].
+          iApply (refines_na_close with "[-]").
+          iFrame.
+          iSplitL.
+          { replace (Z.of_nat q + 1)%Z with (Z.of_nat (q+1)) by lia.
+            iFrame.
+            iModIntro.
+            iPureIntro; split.
+            - rewrite size_dom. rewrite size_dom in dom_q.
+              rewrite map_size_insert_None; first lia.
+              apply not_elem_of_dom_1.
+              rewrite -elem_of_elements.
+              rewrite -Hl'.
+              intros K.
+              apply elem_of_list_fmap_2_inj in K; last apply fin_to_nat_inj.
+              done.
+            - intros x.
+              rewrite elem_of_elements.
+              set_unfold.
+              intros [|]; last naive_solver.
+              subst. apply fin_to_nat_lt.
+          }
+          idtac...
+          rel_values.
+          repeat iExists _.
+          iModIntro. iRight. repeat iSplit ; iPureIntro ; eauto.
+          simpl. repeat unshelve eexists ; try by lia.
+          * assert (r_in <= Input). 2: lia. clear. apply fin.fin_to_nat_le.
+          * cut ((xor_sem (Z.to_nat msg) y < S Output)).
+            1: lia.
+            apply xor_dom ; lia.
+        + iApply (refines_na_close with "[-]").
+          iFrame.
+          iSplit...
+          { done. }
+          rel_values. repeat iExists _. iLeft. done.
+    Qed.
+
+  (* Should be just syntactic since CPA_rand doesn't use the PRF. *)
+  Lemma cpa_F :
+    ⊢ (REL (adversary (CPA_rand sym_scheme_I #Q))
+         << (adversary (CPA_rand sym_scheme_F #Q)) : lrel_bool).
+  Proof with (rel_pures_l ; rel_pures_r).
+    rewrite /sym_scheme_I/sym_scheme_F/I_enc/F_enc/I.
+    rewrite /CPA_rand/symmetric.CPA_rand. idtac...
+    replace lrel_bool with (interp TBool []) by auto.
+    iApply refines_typed. rewrite /F_rand_cipher. tychk.
+    1: apply adversary_typed.
+    rewrite /q_calls_poly. tychk.
+  Qed.
+
+  End approxis_proofs.
+
+  (* Next, we will:
+     - for each step of logical refinement, write the corresponding ARcoupling
+     - chain these together to obtain an ARcoupling for one direction
+     - admit the other direction
+     - combine both directions to get a bound on the difference of observing a #true
+   *)
+
+  Ltac lr_arc := unshelve eapply approximates_coupling ; eauto ;
+                 [apply (λ _, lrel_bool)|try lra|by iIntros (???) "#(%b&->&->)"|iIntros].
+
+  Lemma reduction_ARC Σ `{approxisRGpreS Σ} σ σ' :
+    ARcoupl (lim_exec ((adversary (CPA_real sym_scheme_F #Q)), σ))
+      (lim_exec ((RED' (PRF_real PRF_scheme_F #Q)), σ'))
+      eq 0.
+  Proof using (xor_sem_typed keygen_sem_typed adversary_sem_typed Key H_in_out
+F_sem_typed). lr_arc ; iApply reduction. Qed.
+
+  Lemma F_I_ARC Σ `{approxisRGpreS Σ} σ σ' :
+    ARcoupl (lim_exec ((RED' (PRF_rand PRF_scheme_F #Q)), σ))
+      (lim_exec ((RED' (PRF_rand PRF_scheme_I #Q)), σ'))
+      eq 0.
+  Proof. lr_arc ; iApply F_I. Qed.
+
+  Lemma reduction'_ARC Σ `{approxisRGpreS Σ} σ σ' :
+    ARcoupl (lim_exec ((RED' (PRF_rand PRF_scheme_I #Q)), σ))
+      (lim_exec ((adversary (CPA_real sym_scheme_I #Q)), σ'))
+      eq 0.
+  Proof using (keygen_typed F_typed adversary_typed H_in_out
+                 xor_sem_typed refines_tape_couple_avoid keygen_sem_typed
+                 adversary_sem_typed Key F_sem_typed).
+    lr_arc ; iApply reduction'.
+  Qed.
+
+  Fact ε_Q_pos : (0 <= ε_Q)%R.
+  Proof.
+    repeat apply Rmult_le_pos ; try apply pos_INR.
+    pose proof Rdiv_INR_ge_0 (S Input).
+    cut ((0 <= (2*1) / (2 * INR (S Input))))%R ; first lra.
+    rewrite Rdiv_mult_distr. lra.
+  Qed.
+
+  Lemma cpa_I_ARC Σ `{!approxisRGpreS Σ} (bla : forall (HΣ' : approxisRGS Σ), @XOR_spec Σ HΣ' Message Output H) σ σ' :
+    ARcoupl (lim_exec ((adversary (CPA_real sym_scheme_I #Q)), σ))
+      (lim_exec ((adversary (CPA_rand sym_scheme_I #Q)), σ'))
+      eq ε_Q.
+  Proof using F_typed H_in_out adversary_typed keygen_typed xor_sem_typed
+    refines_tape_couple_avoid keygen_sem_typed adversary_sem_typed Key F_sem_typed.
+    lr_arc. 1: apply ε_Q_pos. iApply cpa_I. iFrame.
+  Qed.
+
+  Lemma cpa_F_ARC Σ `{approxisRGpreS Σ} σ σ' :
+    ARcoupl (lim_exec ((adversary (CPA_rand sym_scheme_I #Q)), σ))
+      (lim_exec ((adversary (CPA_rand sym_scheme_F #Q)), σ'))
+      eq 0.
+  Proof using F_typed H_in_out adversary_typed keygen_typed
+  refines_tape_couple_avoid keygen_sem_typed adversary_sem_typed Key F_sem_typed.
+    lr_arc ; iApply cpa_F. Qed.
+
+  (** The PRF advantage of RED against F. *)
+  Definition ε_F :=
+    advantage (RED' (PRF_real PRF_scheme_F #Q)) (RED' (PRF_rand PRF_scheme_F #Q)) #true.
+
+  (* We will now explore different ways of stating the assumption that F is a
+     PRF. Concretely, we will need to assume that the advantage of the
+     adversary RED, which was constructed by reduction from the adversary
+     against the symmetric scheme, is bounded by some number ε_F. *)
+
+  (* Predicate that states that `ε_F` is an upper bound on the PRF-advantage of
+  `adversary` (in the logical relation!). *)
+  Definition PRF_advantage_upper_bound `{!approxisRGS Σ} (adversary : val) (ε_F : nonnegreal) :=
+    (↯ ε_F ⊢ (REL (adversary (PRF_real PRF_scheme_F #Q)) << (adversary (PRF_rand PRF_scheme_F #Q)) : lrel_bool))
+    /\
+      (↯ ε_F ⊢ (REL (adversary (PRF_rand PRF_scheme_F #Q)) << (adversary (PRF_real PRF_scheme_F #Q)) : lrel_bool)).
+
+  (** This assumption states that owning ↯ ε_F error credits allows to prove
+      the refinement about RED in Approxis. **)
+  Hypothesis H_ε_LR : forall `{approxisRGS Σ},
+      PRF_advantage_upper_bound RED ε_F.
+
+  (* By adequacy, we deduce from the previous assumption that a corresponding
+     approximate refinement coupling holds up to ε_F. *)
+  Fact H_ε_ARC_from_LR Σ `{approxisRGpreS Σ} σ σ' :
+    ARcoupl (lim_exec (RED (PRF_real PRF_scheme_F #Q), σ))
+      (lim_exec (RED (PRF_rand PRF_scheme_F #Q), σ'))
+      eq ε_F.
+  Proof.
+    intros ; lr_arc. 1: apply cond_nonneg. by iApply (proj1 H_ε_LR).
+  Qed.
+
+  (* Alternatively, we can directly make the (weaker) assumption that such an
+     ε_F-ARcoupling exists, since our only use for H_ε_LR is to build this
+     ARcoupling. *)
+  Hypothesis H_ε_ARC :
+    forall σ σ',
+    ARcoupl (lim_exec (RED' (PRF_real PRF_scheme_F #Q), σ))
+      (lim_exec (RED' (PRF_rand PRF_scheme_F #Q), σ'))
+      eq ε_F.
+
+  (* Either way, we can compose the ARC-level reduction lemmas and the
+     assumption H_ε_ARC to get an ARC. *)
+  Lemma prf_cpa_ARC Σ `{approxisRGpreS Σ} σ σ' :
+    ARcoupl (lim_exec ((adversary (CPA_real sym_scheme_F #Q)), σ))
+      (lim_exec ((adversary (CPA_rand sym_scheme_F #Q)), σ'))
+      eq (ε_Q + ε_F).
+  Proof.
+    set (ε := (ε_Q + NNRbar_to_real (NNRbar.Finite ε_F))%R).
+    assert (0 <= ε_F)%R by apply cond_nonneg. pose proof ε_Q_pos.
+    assert (0 <= ε)%R.
+    { unfold ε. apply Rplus_le_le_0_compat ; auto. }
+    replace ε with (0+ε)%R by lra.
+    eapply ARcoupl_eq_trans_l => //.
+    1: eapply reduction_ARC => //.
+    replace ε with (ε_F+ε_Q)%R by (unfold ε ; lra).
+    eapply ARcoupl_eq_trans_l. 1,2 : auto.
+    1: eapply (H_ε_ARC σ σ').
+    replace ε_Q with (0 + ε_Q)%R by lra.
+    eapply ARcoupl_eq_trans_l => //.
+    1: eapply F_I_ARC => //.
+    replace ε_Q with (0 + ε_Q)%R by lra.
+    eapply ARcoupl_eq_trans_l => //.
+    1: eapply reduction'_ARC => //.
+    replace ε_Q with (ε_Q + 0)%R by lra.
+    eapply ARcoupl_eq_trans_l => //.
+    1: eapply cpa_I_ARC => //.
+    1:
+      (* TODO stupid type classes *)
+      admit.
+    eapply cpa_F_ARC => //.
+    Unshelve. all: eauto.
+  Admitted.
+
+  (* The converse direction of the refinement. We expect it to hold with the
+     same bound. *)
+  Variable prf_cpa_ARC' : forall Σ `{approxisRGpreS Σ} σ σ',
+    ARcoupl (lim_exec ((adversary (CPA_rand sym_scheme_F #Q)), σ))
+      (lim_exec ((adversary (CPA_real sym_scheme_F #Q)), σ'))
+      eq (ε_Q + ε_F).
+
+  Corollary CPA_bound_1 Σ `{approxisRGpreS Σ} σ σ' :
+    ( (lim_exec ((adversary (CPA_real sym_scheme_F #Q)), σ) #true)
+      <= (lim_exec ((adversary (CPA_rand sym_scheme_F #Q)), σ') #true)
+         + (ε_Q + ε_F))%R.
+  Proof. apply ARcoupl_eq_elim. by eapply prf_cpa_ARC. Qed.
+
+  Corollary CPA_bound_2 Σ `{approxisRGpreS Σ} σ σ' :
+    ( (lim_exec ((adversary (CPA_rand sym_scheme_F #Q)), σ) #true)
+      <= (lim_exec ((adversary (CPA_real sym_scheme_F #Q)), σ') #true)
+         + (ε_Q + ε_F))%R.
+  Proof using prf_cpa_ARC'. apply ARcoupl_eq_elim. by eapply prf_cpa_ARC'. Qed.
+
+  Theorem CPA_bound_st Σ `{approxisRGpreS Σ} σ σ' :
+    (pr_dist (adversary (CPA_real sym_scheme_F #Q)) (adversary (CPA_rand sym_scheme_F #Q)) σ σ' #true
+     <= ε_Q + ε_F)%R.
+  Proof using F_typed H_in_out H_ε_ARC H_ε_LR adversary_typed keygen_typed prf_cpa_ARC'
+  refines_tape_couple_avoid keygen_sem_typed adversary_sem_typed Key F_sem_typed.
+    apply Rabs_le.
+    pose proof CPA_bound_1 Σ σ σ'.
+    pose proof CPA_bound_2 Σ σ' σ.
+    set (lhs := lim_exec (adversary (CPA_real sym_scheme_F #Q), σ) #true).
+    set (rhs := lim_exec (adversary (CPA_rand sym_scheme_F #Q), σ') #true).
+    assert (lhs <= rhs + (ε_Q + ε_F))%R by easy.
+    assert (rhs <= lhs + (ε_Q + ε_F))%R by easy.
+    split ; lra.
+  Qed.
+
+  (** Instead of making an assumption about F at the ARcoupl level, we can work
+  directly with pr_dist. Since ε_F is defined to be the advantage, no further
+  assumptions are needed. We prove the (ε_Q+ε_F) bound by lowering all the
+  reduction lemmas to the pr_dist level and composing there. **)
+
+  (* Reduce from CPA security to a statement about PRF security of F (real side) *)
+  Lemma red_to_prf Σ `{approxisRGpreS Σ} σ σ' :
+    ARcoupl (lim_exec (adversary (CPA_real sym_scheme_F #Q), σ))
+      (lim_exec ((RED' (PRF_real PRF_scheme_F #Q)), σ')) eq 0%R.
+  Proof using keygen_sem_typed adversary_sem_typed Key H_in_out
+F_sem_typed xor_sem_typed.
+    eapply reduction_ARC => //. Qed.
+
+  (* The reverse direction *)
+  Hypothesis red_to_prf' : forall Σ `{approxisRGpreS Σ} σ σ',
+    ARcoupl (lim_exec ((RED' (PRF_real PRF_scheme_F #Q)), σ'))
+      (lim_exec (adversary (CPA_real sym_scheme_F #Q), σ)) eq 0%R.
+
+  (* Combine to get the pr_dist bound. *)
+  Lemma pr_dist_adv_F `{approxisRGpreS Σ} v σ σ' :
+    (pr_dist (adversary (CPA_real sym_scheme_F #Q)) (RED' (PRF_real PRF_scheme_F #Q)) σ σ' v
+     <= 0)%R.
+  Proof using xor_sem_typed red_to_prf' keygen_sem_typed adversary_sem_typed Key
+    H_in_out F_sem_typed.
+    rewrite /pr_dist.
+    eapply Rabs_le.
+    split.
+    - opose proof (ARcoupl_eq_elim _ _ _ (red_to_prf' _ σ σ') v) as hred.
+      set (y := (lim_exec (adversary _, σ)) v).
+      set (x := lim_exec (RED' _, σ') v).
+      assert (x <= y + 0)%R by easy.
+      lra.
+    - opose proof (ARcoupl_eq_elim _ _ _ (red_to_prf _ σ σ') v) as hred.
+      set (x := (lim_exec (adversary _, σ)) v).
+      set (y := lim_exec (RED' _, σ') v).
+      assert (x <= y + 0)%R by easy.
+      lra.
+  Qed.
+
+  (* Reduce from CPA security to a statement about PRF security of F (rand side) *)
+  Lemma red_from_prf Σ `{approxisRGpreS Σ} σ σ' :
+    ARcoupl (lim_exec (RED' (PRF_rand PRF_scheme_F #Q), σ))
+      (lim_exec (adversary (CPA_rand sym_scheme_F #Q), σ'))
+      eq ε_Q.
+  Proof.
+    pose proof ε_Q_pos.
+    replace ε_Q with (0 + ε_Q)%R by lra.
+    eapply ARcoupl_eq_trans_l => //.
+    1: eapply (F_I_ARC _ _ σ) => //.
+    replace ε_Q with (0 + ε_Q)%R by lra.
+    eapply ARcoupl_eq_trans_l => //.
+    1: eapply (reduction'_ARC _ _ σ) => //.
+    replace ε_Q with (ε_Q + 0)%R by lra.
+    eapply ARcoupl_eq_trans_l => //.
+    1: eapply (cpa_I_ARC _ _ _ σ) => //.
+    eapply cpa_F_ARC => //.
+    Unshelve. all: eauto.
+    admit.                      (* TODO stupid type classes again *)
+  Admitted.
+
+  (* The reverse direction *)
+  Hypothesis red_from_prf' : forall Σ `{approxisRGpreS Σ} σ σ',
+    ARcoupl (lim_exec (adversary (CPA_rand sym_scheme_F #Q), σ'))
+      (lim_exec (RED' (PRF_rand PRF_scheme_F #Q), σ))
+      eq ε_Q.
+
+  (* Combine to get the pr_dist bound. *)
+  Lemma pr_dist_F_adv `{approxisRGpreS Σ} v σ σ' :
+    (pr_dist (RED' (PRF_rand PRF_scheme_F #Q)) (adversary (CPA_rand sym_scheme_F #Q)) σ σ' v
+     <= ε_Q)%R.
+  Proof.
+    rewrite /pr_dist. eapply Rabs_le. split.
+    - opose proof (ARcoupl_eq_elim _ _ _ (red_from_prf' _ σ σ') v) as hred.
+      set (x := lim_exec (RED' _, σ) v).
+      set (y := (lim_exec (adversary _, σ')) v).
+      assert (y <= x + ε_Q)%R by easy. lra.
+    - opose proof (ARcoupl_eq_elim _ _ _ (red_from_prf _ σ σ') v) as hred.
+      set (x := lim_exec (RED' _, σ) v).
+      set (y := (lim_exec (adversary _, σ')) v).
+      assert (x <= y + ε_Q)%R by easy. lra.
+  Qed.
+
+  (* Same statement as CPA_bound_st but proven without assuming H_ε_ARC or H_ε_LR. *)
+  Theorem CPA_bound_st' Σ `{approxisRGpreS Σ} σ σ' :
+    (pr_dist (adversary (CPA_real sym_scheme_F #Q)) (adversary (CPA_rand sym_scheme_F #Q)) σ σ' #true
+     <= ε_Q + ε_F)%R.
+  Proof using xor_sem_typed refines_tape_couple_avoid red_to_prf'
+    red_from_prf' prf_cpa_ARC' keygen_typed keygen_sem_typed adversary_typed
+    adversary_sem_typed Key H_ε_LR H_ε_ARC H_in_out F_typed F_sem_typed.
+    eapply pr_dist_triangle.
+    1: eapply pr_dist_adv_F.
+    1: eapply pr_dist_triangle.
+    2: eapply pr_dist_F_adv.
+    1: eapply (advantage_ub).
+    1: right ; eauto.
+    unfold ε_Q, ε_F. lra.
+  Qed.
+
+  Theorem CPA_bound Σ `{approxisRGpreS Σ} :
+    (advantage
+       (adversary (CPA_real sym_scheme_F #Q))
+       (adversary (CPA_rand sym_scheme_F #Q))
+       #true
+     <= ε_Q + ε_F)%R.
+  Proof using Cipher F F_keygen F_sem_typed F_typed H H_in_out H_ε_ARC H_ε_LR
+    Input Key Message Output Q adversary adversary_sem_typed adversary_typed
+    keygen keygen_sem_typed keygen_typed prf_cpa_ARC' refines_tape_couple_avoid
+    ε_Q.
+    apply advantage_uniform.
+    by eapply CPA_bound_st => //.
+  Qed.
+
+  (* TODO Something about PPT and proving that if (isNegligable ε_F) then also
+     (isNegligable (ε_F + ε_Q))... *)
+  Variable PPT : expr → Prop.
+  Hypothesis adv_in_PPT : PPT adversary.
+  Hypothesis RED_in_PPT : PPT adversary → PPT RED.
+
+  (*
+
+Recall that a function f is negligible if any n, there exists M_n, s.t. for all
+λ > M_n, f(λ) < 1/λ^n.
+
+Definition (Advantage).
+
+The distinguishing advantage between two programs X and Y is defined as
+
+advantage(X, Y) = max_(σ,σ') | lim_exec(X,σ)(true) - lim_exec(Y,σ')(true) | .
+
+
+Nota bene: In security statements, X and Y are typically of the form (A G_real)
+and (A G_rand), but in security reductions they may, for instance, be of the
+form (A G_real) and (RED H_rand) so rather than defining the advantage for a
+fixed adversary and two games, we instead define it directly for two programs.
+
+
+Definition (PRF security).
+
+Let F = (F)_λ be a family of functions indexed by a security parameter λ. F is
+a secure PRF if for all adversaries A, if A is PPT, then the function
+
+    f(λ) = advantage (A λ (PRF_real (F λ))) (A λ (PRF_rand (F λ)))
+
+is negligible.
+
+
+Definition (IND$-CPA security).
+
+Let Σ = (Σ)_λ be a family of symmetric encryption schemes indexed by a security
+parameter λ. Σ has IND$-CPA security if for all adversaries A, if A is PPT,
+then the function
+
+    f(λ) = advantage (A λ (IND$_CPA_real (Σ λ))) (A λ (IND$_CPA_rand (Σ λ)))
+
+is negligible.
+
+
+The theorem CPA_bound states that for any function F, the IND$-CPA advantage of
+any adversary A is bounded by ε = ε_F + ε_Q, where ε_Q = Q²/2N and ε_F is the
+PRF advantage of A against F [TODO "the PRF advantage of A" is undefined]
+
+If we want to conclude that Σ_F is secure against PPT CPA adversaries because F
+is, then we need to use the fact that RED is a PPT PRF adversary.
+[TODO spell this out]
+
+Note, however, that the PPT assumption plays no role in the concrete security
+setting. When λ is fixed to, say, 2048 bits, and ε_F is e.g. 1/2^128, then the
+ε_F + ε_Q bound
+
+   *)
+
+
+
+End combined.
